src/tls/TLSExtensions_Redux.fst
@@ -1,0 +1,568 @@
+﻿(*--build-config
+  options:--codegen-lib CoreCrypto --codegen-lib Platform --codegen-lib Classical --codegen-lib SeqProperties --codegen-lib HyperHeap  --admit_fsi FStar.Char --admit_fsi FStar.HyperHeap --admit_fsi FStar.Set --admit_fsi FStar.Map --admit_fsi FStar.Seq --admit_fsi SessionDB --admit_fsi UntrustedCert --admit_fsi DHDB --admit_fsi CoreCrypto --admit_fsi Cert --admit_fsi Handshake --max_fuel 4 --initial_fuel 0 --max_ifuel 2 --initial_ifuel 1 --z3timeout 5 --lax;
+  other-files:ext.fst classical.fst FStar.Set.fsi FStar.Heap.fst map.fsi listTot.fst hyperHeap.fsi stHyperHeap.fst allHyperHeap.fst char.fsi string.fst list.fst listproperties.fst seq.fsi seqproperties.fst /home/jkz/dev/FStar/contrib/Platform/fst/Bytes.fst /home/jkz/dev/FStar/contrib/Platform/fst/Date.fst /home/jkz/dev/FStar/contrib/Platform/fst/Error.fst /home/jkz/dev/FStar/contrib/Platform/fst/Tcp.fst /home/jkz/dev/FStar/contrib/CoreCrypto/fst/CoreCrypto.fst /home/jkz/dev/FStar/contrib/CoreCrypto/fst/DHDB.fst TLSError.fst TLSConstants-redux.fst Nonce.fst RSAKey.fst DHGroup.p.fst ECGroup.fst CommonDH.fst PMS.p.fst HASH.fst HMAC.fst Sig.p.fst UntrustedCert.fsti Cert.fsti TLSInfo.fst;
+  --*)
+
+(* Copyright (C) 2012--2015 Microsoft Research and INRIA *)
+
+#light "off"
+
+module TLSExtensions
+
+open Platform.Bytes
+open Platform.Error
+open TLSError
+open TLSConstants
+open TLSInfo
+open CoreCrypto
+
+type preEarlyDataIndication =
+  { ped_configuration_id: configuration_id;
+    ped_cipher_suite:cipherSuite;
+    ped_extensions:list extension;
+    ped_content:bytes;
+    ped_early_data_type:earlyDataType; }
+and earlyDataIndication = 
+  | ClientEarlyDataIndication of preEarlyDataIndication 
+  | ServerEarlyDataIndication
+// JK : can I merge client extensions and server extensions ?
+and extension = 
+  // TLS 1.3 extension types
+  | E_earlyData of earlyDataIndication // JK : TODO : put appropriate type
+  | E_preSharedKey of preSharedKey // JK : TODO : put appropriate type
+  | E_keyShare of keyShare // JK : TODO : put appropriate type
+  // Common extension types
+  | E_signatureAlgorithms of (list sigHashAlg) // JK : TODO : put appropriate type, did it previously appear ?
+  // Previous extension types
+  | E_renegotiation_info of (cVerifyData * option sVerifyData) // JK : option is some if server side
+  | E_server_name of list serverName
+  | E_extended_ms 
+  | E_extended_padding 
+  | E_ec_point_format of list ECGroup.point_format
+  | E_supported_groups of list namedGroup
+  | E_unknown_extension of (lbytes 2 * bytes) // Still store unknown extension to get parsing injectivity
+
+let sameExt a b =
+  match a, b with
+  | E_earlyData _, E_earlyData _ -> true
+  | E_preSharedKey _, E_preSharedKey _ -> true
+  | E_keyShare _, E_keyShare _ -> true
+  | E_signatureAlgorithms _, E_signatureAlgorithms _ -> true
+  | E_renegotiation_info _, E_renegotiation_info _ -> true 
+  | E_server_name _, E_server_name _ -> true
+  | E_extended_ms, E_extended_ms -> true 
+  | E_extended_padding, E_extended_padding -> true 
+  | E_ec_point_format _, E_ec_point_format _ -> true
+  | E_supported_groups _, E_supported_groups _ -> true
+  | _ -> false
+
+val extensionHeaderBytes: extension -> Tot bytes
+let extensionHeaderBytes ext =
+  match ext with
+  | E_earlyData _           -> abyte2 (0x00uy, 0x02uy) // JK : TODO, TBD
+  | E_preSharedKey _        -> abyte2 (0x00uy, 0x03uy) // JK : TODO, TBD
+  | E_keyShare _            -> abyte2 (0x00uy, 0x04uy) // JK : TODO, TBD
+  | E_signatureAlgorithms _ -> abyte2 (0x00uy, 0x0Duy)
+  | E_renegotiation_info(_) -> abyte2 (0xFFuy, 0x01uy)
+  | E_server_name (_)       -> abyte2 (0x00uy, 0x00uy)
+  | E_extended_ms           -> abyte2 (0x00uy, 0x17uy)
+  | E_extended_padding      -> abyte2 (0xBBuy, 0x8Fuy)
+  | E_ec_point_format _     -> abyte2 (0x00uy, 0x0Buy)
+  | E_supported_groups _    -> abyte2 (0x00uy, 0x0Auy)
+  | E_unknown_extension(h,b)-> h
+
+type CanFail (a:Type) =
+| ExFail of alertDescription * string
+| ExOK of list a
+
+val compile_sni_list: list serverName -> Tot bytes
+let compile_sni_list l =
+    let rec (aux:list serverName -> Tot bytes) = function
+    | [] -> empty_bytes
+    | SNI_DNS(x) :: r -> (abyte 0uy) @| bytes_of_int 2 (length x) @| x @| aux r
+    | SNI_UNKNOWN(t, x) :: r -> (bytes_of_int 1 t) @| bytes_of_int 2 (length x) @| x @| aux r
+    in aux l
+
+val parse_sni_list: b:bytes -> Tot (Result (list serverName))
+let parse_sni_list b  =
+    let rec (aux:bytes -> Tot (CanFail (serverName))) = fun b ->
+        if equalBytes b empty_bytes then ExOK([])
+        else
+            let (ty,v) = split b 1 in
+            (match vlsplit 2 v with
+            | Error(x,y) -> ExFail(x,y)
+            | Correct(cur, next) ->
+                (match aux next with
+                | ExFail(x,y) -> ExFail(x,y)
+                | ExOK(l) ->
+		    admit();
+                    let cur =
+                        (match cbyte ty with
+                        | 0uy -> SNI_DNS(cur)
+                        | v -> SNI_UNKNOWN(int_of_bytes ty, cur))
+                    in let (snidup:serverName -> Tot bool) = fun x ->
+                        (match (x,cur) with
+                        | SNI_DNS _, SNI_DNS _ -> true
+                        | SNI_UNKNOWN(a,_), SNI_UNKNOWN(b, _) when (a=b) -> true
+                        | _ -> false)
+		       in if List.existsb snidup l then ExFail(AD_unrecognized_name, perror __SOURCE_FILE__ __LINE__ "Duplicate SNI type")
+                    else ExOK(cur :: l)))
+    in (match aux b with
+    | ExFail(x,y) -> Error(x,y)
+    | ExOK([]) -> Error(AD_unrecognized_name, perror __SOURCE_FILE__ __LINE__ "Empty SNI extension")
+    | ExOK(l) -> correct (l))
+
+val compile_curve_list: list ECGroup.ec_all_curve -> Tot bytes
+let compile_curve_list l =
+    let rec (aux:list ECGroup.ec_all_curve -> Tot bytes) =
+        function
+        | [] -> empty_bytes
+        | ECGroup.EC_CORE c :: r ->
+            let cid = ECGroup.curve_id (ECGroup.getParams c) in
+            cid @| aux r
+        | ECGroup.EC_EXPLICIT_PRIME :: r -> abyte2 (255uy, 01uy) @| aux r
+        | ECGroup.EC_EXPLICIT_BINARY :: r -> abyte2 (255uy, 02uy) @| aux r
+        | ECGroup.EC_UNKNOWN(x) :: r -> bytes_of_int 2 x @| aux r
+    in
+    let al = aux l in
+    let bl: bytes = vlbytes 2 al in
+    bl
+
+val parse_curve_list: bytes -> Tot (Result (list ECGroup.ec_all_curve))
+let parse_curve_list b =
+    let rec (aux:bytes -> Tot (CanFail ECGroup.ec_all_curve)) = fun b ->
+        if equalBytes b empty_bytes then ExOK([])
+        else if (length b) % 2 = 1 then ExFail(AD_decode_error, perror __SOURCE_FILE__ __LINE__ "Bad encoding of curve list")
+        else let (u,v) = split b 2 in
+            (match aux v with
+            | ExFail(x,y) -> ExFail(x,y)
+            | ExOK(l) ->
+                let cur =
+                    (match cbyte2 u with
+                    | (0uy, 23uy) -> ECGroup.EC_CORE CoreCrypto.ECC_P256
+                    | (0uy, 24uy) -> ECGroup.EC_CORE CoreCrypto.ECC_P384
+                    | (0uy, 25uy) -> ECGroup.EC_CORE CoreCrypto.ECC_P521
+                    | (255uy, 1uy) -> ECGroup.EC_EXPLICIT_PRIME
+                    | (255uy, 2uy) -> ECGroup.EC_EXPLICIT_BINARY
+                    | _ -> ECGroup.EC_UNKNOWN(int_of_bytes u))
+                in
+                    if List.mem cur l then ExFail(AD_decode_error, perror __SOURCE_FILE__ __LINE__ "Duplicate curve")
+                    else ExOK(cur :: l))
+    in (match aux b with
+    | ExFail(x,y) -> Error(x,y)
+    | ExOK([]) -> Error(AD_decode_error, perror __SOURCE_FILE__ __LINE__ "Empty supported curve list")
+    | ExOK(l) -> correct (l))
+
+val parse_ecpf_list: bytes -> (Result (list ECGroup.point_format))
+let parse_ecpf_list b =
+    let rec aux b =
+        if equalBytes b empty_bytes then ExOK([])
+        else let (u,v) = split b 1 in
+            (match aux v with
+            | ExFail(x,y) -> ExFail(x,y)
+            | ExOK(l) ->
+                let cur = match cbyte u with
+                | 0uy -> ECGroup.ECP_UNCOMPRESSED
+                | _ -> ECGroup.ECP_UNKNOWN(int_of_bytes u)
+                in ExOK(cur :: l))
+    in (match aux b with
+    | ExFail(x,y) -> Error(x,y)
+    | ExOK(l) when not (List.mem ECGroup.ECP_UNCOMPRESSED l) ->
+        Error(AD_decode_error, perror __SOURCE_FILE__ __LINE__ "Uncompressed point format not supported")
+    | ExOK(l) -> correct (l))
+
+val compile_ecpf_list: list ECGroup.point_format -> Tot bytes
+let compile_ecpf_list l =
+    let rec (aux:list ECGroup.point_format -> Tot bytes) =
+        function
+        | [] -> empty_bytes
+        | ECGroup.ECP_UNCOMPRESSED :: r -> (abyte 0uy) @| aux r
+        | ECGroup.ECP_UNKNOWN(t) :: r -> (bytes_of_int 1 t) @| aux r
+    in
+    let al = aux l in
+    let bl:bytes = vlbytes 1 al in
+    bl
+
+
+val earlyDataIndicationBytes: earlyDataIndication -> Tot bytes
+val extensionPayloadBytes: extension -> Tot bytes
+val extensionBytes: extension -> Tot bytes
+val extensionsBytes: cl:list extension -> Tot (b:bytes{length b < ((List.length cl) * 65539)})
+let rec earlyDataIndicationBytes edi =
+  match edi with
+  | ServerEarlyDataIndication -> empty_bytes
+  | ClientEarlyDataIndication edi ->
+      let cid_bytes = configurationIdBytes edi.ped_configuration_id in
+      let cs_bytes = cipherSuiteBytes edi.ped_cipher_suite in
+      let ext_bytes = extensionsBytes edi.ped_extensions in
+      let content_bytes = vlbytes 1 edi.ped_content in
+      let edt_bytes = earlyDataTypeBytes edi.ped_early_data_type in
+      cid_bytes @| cs_bytes @| ext_bytes @| content_bytes @| edt_bytes
+and extensionPayloadBytes ext =
+  match ext with
+  | E_earlyData edt           -> earlyDataIndicationBytes edt
+  | E_preSharedKey psk        -> preSharedKeyBytes psk
+  | E_keyShare ks             -> keyShareBytes ks
+  | E_signatureAlgorithms sha -> sigHashAlgsBytes sha
+  | E_renegotiation_info(cvd, svd) -> 
+    (match svd with | None -> vlbytes 1 cvd | Some svd' -> let p = cvd @| svd' in vlbytes 1 p)
+  | E_server_name(l) -> compile_sni_list l
+  | E_extended_ms -> empty_bytes
+  | E_extended_padding -> empty_bytes
+  | E_supported_groups(l) -> namedGroupsBytes l
+  | E_ec_point_format(l) -> compile_ecpf_list l
+  | E_unknown_extension(h,b) -> b
+and extensionBytes ext =
+    let head = extensionHeaderBytes ext in
+    let payload = extensionPayloadBytes ext in
+    let payload = vlbytes 2 payload in
+    head @| payload
+and extensionsBytes exts =
+  List.fold_leftT (fun l s -> l @| extensionBytes s) empty_bytes exts
+
+(*
+let parseExtension head payload role =
+    match cbyte2 head with
+    | (0uy, 0uy) -> // Server name indication
+        (match vlparse 2 payload with
+        | Error (x,y) -> Some(Error(x,y))
+        | Correct(sni) ->
+            (match parse_sni_list sni with
+            | Error (x,y) -> Some(Error(x,y))
+            | Correct(l) -> Some(correct (E_server_name(l)))))
+    | (0xFFuy, 0x01uy) -> // renegotiation info
+        (match vlparse 1 payload with
+        | Error (x,y) -> Some(Error(x,y))
+        | Correct(vd) ->
+	  (match role with 
+	   | Client ->
+            (let res = E_renegotiation_info (vd,None) in
+            let res = correct res in
+            Some(res))
+	   | Server -> 
+	    (let vdL = length vd in
+	    let (cvd, svd) = split vd (vdL/2) in
+	    let res = E_renegotiation_info(cvd,Some svd) in
+	    let res = correct res in
+	    Some res)))
+    | (0x00uy, 0x0Auy) -> // Supported EC curves
+        (match vlparse 2 payload with
+        | Error (x,y) -> Some(Error(x,y))
+        | Correct(ecl) ->
+            (match parse_curve_list ecl with
+            | Error (x,y) -> Some(Error(x,y))
+            | Correct(l) -> Some(correct (E_supported_groups(l)))))
+    | (0x00uy, 0x0Buy) -> // Supported EC point formats
+        (match vlparse 1 payload with
+        | Error (x,y) -> Some(Error(x,y))
+        | Correct(ecpf) ->
+            (match parse_ecpf_list ecpf with
+            | Error (x,y) -> Some(Error(x,y))
+            | Correct(l) -> Some(correct (E_ec_point_format(l)))))
+#if TLSExt_sessionHash
+    | (0x00uy, 0x17uy) -> // extended_ms
+        if equalBytes payload empty_bytes then
+            Some(correct (E_extended_ms))
+        else
+            Some(Error(AD_illegal_parameter, perror __SOURCE_FILE__ __LINE__ "Invalid data for extended master secret extension"))
+#endif
+#if TLSExt_extendedPadding
+    | (0xBBuy, 0x8Fuy) -> // extended_padding
+        if equalBytes payload empty_bytes then
+            Some(correct (E_extended_padding))
+        else
+            Some(Error(AD_illegal_parameter, perror __SOURCE_FILE__ __LINE__ "Invalid data for extended padding extension"))
+#endif
+    // JK : used to be skipped, now stored as "unknown extension"
+    | (_,_) -> Some (correct (E_unknown_extension (head @| payload)))
+
+let addOnce ext extList =
+    if List.existsb (sameExt ext) extList then
+        Error(AD_handshake_failure, perror __SOURCE_FILE__ __LINE__ "Same extension received more than once")
+    else
+        let res = ext::extList in
+        correct(res)
+
+let rec parseExtensionList ext extList role =
+    match length ext with
+    | 0 -> correct (extList)
+    | x when (x < 4) ->
+        (* This is a parsing error, or a malformed extension *)
+        Error (AD_decode_error, perror __SOURCE_FILE__ __LINE__ "")
+    | _ ->
+        let (extTypeBytes,rem) = Platform.Bytes.split ext 2 in
+        match vlsplit 2 rem with
+            | Error(x,y) -> Error (x,y) (* Parsing error *)
+            | Correct (res) ->
+                let (payload,rem) = res in
+                match parseExtension extTypeBytes payload role with
+                | None ->
+		    // JK : this case does not happen anymore
+                    (* Unknown extension, skip it *)
+                    parseExtensionList rem extList role		    
+                | Some(res) ->
+                    match res with
+                    | Error(x,y) -> Error(x,y)
+                    | Correct(ce) ->
+                        match addOnce ce extList with
+                        | Error(x,y) -> Error(x,y)
+                        | Correct(extList) -> parseExtensionList rem extList role
+
+let rec parseSCSVs ch_ciphers extL =
+    if contains_TLS_EMPTY_RENEGOTIATION_INFO_SCSV ch_ciphers then
+        addOnce (E_renegotiation_info(empty_bytes, None)) extL
+    else
+        correct(extL)
+
+val parseExtensions: data:bytes -> known_cipher_suites -> role -> Result (list extension)
+let parseExtensions data ch_ciphers role =
+    match length data with
+    | 0 -> parseSCSVs ch_ciphers []
+    | 1 -> Error(AD_decode_error, perror __SOURCE_FILE__ __LINE__ "")
+    | _ ->
+        match vlparse 2 data with
+        | Error(x,y)    -> Error(x,y)
+        | Correct(exts) ->
+            match parseExtensionList exts [] role with
+            | Error(x,y) -> Error(x,y)
+            | Correct(extL) -> parseSCSVs ch_ciphers extL
+
+// JK : Only client side ? 
+val prepareExtensions: config -> ConnectionInfo -> cVerifyData -> l:list extension{List.length l < 256}
+let prepareExtensions (cfg:config) (conn:ConnectionInfo) renegoCVD =
+    (* Always send supported extensions. The configuration options will influence how strict the tests will be *)
+    let res = [E_renegotiation_info(renegoCVD, None)] in
+#if TLSExt_sessionHash
+    let res = E_extended_ms :: res in
+#endif
+#if TLSExt_extendedPadding
+    let res = E_extended_padding :: res in
+#endif
+    let res =
+        let curves = List.map (fun x -> ECGroup.EC_CORE x) cfg.ecdhGroups in
+        if curves <> [] && List.existsb (fun x -> isECDHECipherSuite x) cfg.ciphersuites then
+            E_ec_point_format([ECGroup.ECP_UNCOMPRESSED]) :: E_supported_groups(curves) :: res
+        else res in
+    res
+
+let serverToNegotiatedExtension cExtL (resuming:bool) cs res sExt : Result (negotiatedExtensions)=
+    match res with
+    | Error(x,y) -> Error(x,y)
+    | Correct(l) ->
+        if List.existsb (sameExt sExt) cExtL then
+            match sExt with
+            | E_renegotiation_info (cvd,svd) -> 
+	      (match svd with
+	      | Some svd' -> correct ({l with ne_renegotiation_info=Some(cvd,svd')})
+	      | None -> Error(AD_handshake_failure,perror __SOURCE_FILE__ __LINE__ "Server sent renegotiation info without server verified data"))
+            | E_server_name _ ->
+                if List.existsb (fun x->match x with E_server_name _ -> true | _ -> false) cExtL then correct(l)
+                else Error(AD_handshake_failure,perror __SOURCE_FILE__ __LINE__ "Server sent an SNI acknowledgement without an SNI provided")
+            | E_ec_point_format(spf) ->
+                if resuming then
+                    correct l
+                else
+                    correct ({l with ne_supported_point_formats = Some spf})
+            | E_extended_ms ->
+                if resuming then
+                    correct(l)
+                else
+                    correct({l with ne_extended_ms = true})
+            | E_extended_padding ->
+                if resuming then
+                    Error(AD_handshake_failure,perror __SOURCE_FILE__ __LINE__ "Server provided extended padding in a resuming handshake")
+                else
+                    if isOnlyMACCipherSuite cs then
+                        Error(AD_handshake_failure,perror __SOURCE_FILE__ __LINE__ "Server provided extended padding for a MAC only ciphersuite")
+                    else
+                        correct({l with ne_extended_padding = true})
+        else
+            Error(AD_handshake_failure,perror __SOURCE_FILE__ __LINE__ "Server provided an extension not given by the client")
+
+let negotiateClientExtensions (cExtL:list extension) (sExtL:list extension) (resuming:bool) cs =
+    let nes = ne_default in
+    match List.fold_left (serverToNegotiatedExtension cExtL resuming cs) (correct nes) sExtL with
+    | Error(x,y) -> Error(x,y)
+    | Correct(l) ->
+        // Client-side specific extension negotiation
+        // Nothing for now
+        correct(l)
+
+let clientToServerExtension (cfg:config) (cs:cipherSuite) ((renegoCVD:cVerifyData),(renegoSVD:sVerifyData)) (resuming:bool) (cExt:extension) : (option (extension)) =
+    match cExt with
+    | E_earlyData b -> None    // JK : how to handle these here ?
+    | E_preSharedKey b -> None // JK : how to handle these here ?
+    | E_keyShare b -> None     // JK : how to handle these here ?
+    | E_renegotiation_info (_) -> Some (E_renegotiation_info (renegoCVD,renegoSVD))
+    | E_server_name l ->
+        (match List.tryFind (fun x->match x with SNI_DNS _ -> true | _ -> false) l with
+        | Some _ -> Some(E_server_name l)
+        | _ -> None)
+    | E_ec_point_format(l) ->
+        if resuming then None
+        else Some(E_ec_point_format [ECGroup.ECP_UNCOMPRESSED])
+    | E_supported_groups(l) -> None
+    | E_extended_ms -> Some(E_extended_ms)
+    | E_extended_padding ->
+        if resuming then
+            None
+        else
+            if isOnlyMACCipherSuite cs then
+                None
+            else
+                Some(E_extended_padding)
+    | E_unknown_extension b -> None
+    
+
+let clientToNegotiatedExtension (cfg:config) cs ((cvd:cVerifyData),(svd:sVerifyData)) (resuming:bool)  neg cExt =
+    match cExt with
+    | E_renegotiation_info (_) -> {neg with ne_renegotiation_info=Some(cvd,svd)}
+    | E_supported_groups l ->
+        if resuming then neg
+        else
+            let rec okcurves = function
+            | ECGroup.EC_CORE(x) :: r ->
+                let rl = okcurves r in
+                if List.existsb (fun x -> x = x) cfg.ecdhGroups then x::rl else rl
+            | x :: r -> okcurves r
+            | [] -> [] in
+            {neg with ne_supported_curves = Some (okcurves l)}
+    | E_ec_point_format l ->
+        if resuming then neg
+        else
+            let nl = List.filter (fun x -> x = ECGroup.ECP_UNCOMPRESSED) l in
+            {neg with ne_supported_point_formats = Some nl}
+    | E_server_name l ->
+        {neg with ne_server_names = Some l}
+    | E_extended_ms ->
+        if resuming then
+            neg
+        else
+            {neg with ne_extended_ms = true}
+    | E_extended_padding ->
+        if resuming then
+            neg
+        else
+            if isOnlyMACCipherSuite cs then
+                neg
+            else
+                {neg with ne_extended_padding = true}
+    | _ -> neg // JK : handle remaining cases
+
+let negotiateServerExtensions cExtL cfg cs (cvd,svd) resuming  :  (list extension * negotiatedExtensions) =
+    let server = List.choose (clientToServerExtension cfg cs (cvd,svd) resuming) cExtL in
+    let negi = ne_default in
+    let nego = List.fold_left (clientToNegotiatedExtension cfg cs (cvd,Some.v svd) resuming) negi cExtL in
+    (server,nego)
+
+let isClientRenegotiationInfo e =
+    match e with
+    | E_renegotiation_info(cvd, None) -> Some(cvd)
+    | _ -> None
+
+let checkClientRenegotiationInfoExtension config (cExtL: list extension) cVerifyData =
+    match List.tryPick isClientRenegotiationInfo cExtL with
+    | None -> not (config.safe_renegotiation)
+    | Some(payload) -> equalBytes payload cVerifyData
+
+let isServerRenegotiationInfo e =
+    match e with
+    | E_renegotiation_info (cvd,Some svd) -> Some((cvd,svd))
+    | _ -> None
+
+let checkServerRenegotiationInfoExtension config (sExtL: list extension) cVerifyData sVerifyData =
+    match List.tryPick isServerRenegotiationInfo sExtL with
+    | None -> not (config.safe_renegotiation)
+    | Some(x) ->
+        let (cvd,svd) = x in
+        equalBytes (cvd @| svd) (cVerifyData @| sVerifyData)
+
+let hasExtendedMS extL = extL.ne_extended_ms = true
+
+let hasExtendedPadding id = id.ext.ne_extended_padding = true
+
+(* sigHashAlg parsing functions *)
+let sigHashAlgBytes alg =
+    // pre: we're in TLS 1.2
+    let (sign,hash) = alg in
+    let signB = sigAlgBytes sign in
+    let hashB = hashAlgBytes hash in
+    hashB @| signB
+
+let parseSigHashAlg b =
+    let (hashB,signB) = Platform.Bytes.split b 1 in
+    match parseSigAlg signB with
+    | Error(x,y) -> Error(x,y)
+    | Correct(sign) ->
+        match parseHashAlg hashB with
+        | Error(x,y) -> Error(x,y)
+        | Correct(hash) -> correct(sign,hash)
+
+assume val sigHashAlgListBytes: sal:list Sig.alg -> Tot (lbytes (2* List.length sal))
+(*
+let rec sigHashAlgListBytes algL =
+    match algL with
+    | [] -> empty_bytes
+    | h::t ->
+        let oneItem = sigHashAlgBytes h in
+        oneItem @| sigHashAlgListBytes t
+*)
+let rec parseSigHashAlgList b : (Result (list Sig.alg))=
+    if length b = 0 then correct([])
+    else if length b = 1 then Error(AD_decode_error, perror __SOURCE_FILE__ __LINE__ "")
+    else
+        let (thisB,remB) = Platform.Bytes.split b 2 in
+        match parseSigHashAlgList remB with
+        | Error(x,y) -> Error(x,y)
+        | Correct(rem) ->
+            match parseSigHashAlg thisB with
+            | Error(x,y) -> // skip this one
+                correct(rem)
+            | Correct(this) ->
+                correct(this :: rem)
+
+let default_sigHashAlg_fromSig pv sigAlg=
+    match sigAlg with
+    | RSASIG ->
+        (match pv with
+        | TLS_1p2 -> [(RSASIG, Hash SHA1)]
+        | TLS_1p0 | TLS_1p1 | SSL_3p0 -> [(RSASIG,MD5SHA1)])
+        //| SSL_3p0 -> [(RSASIG,NULL)]
+    | DSA ->
+        [(DSA,Hash SHA1)]
+        //match pv with
+        //| TLS_1p0| TLS_1p1 | TLS_1p2 -> [(DSA, SHA1)]
+        //| SSL_3p0 -> [(DSA,NULL)]
+    | _ -> unexpected "[default_sigHashAlg_fromSig] invoked on an invalid signature algorithm"
+
+val default_sigHashAlg: ProtocolVersion -> cipherSuite -> l:list Sig.alg{List.length l <= 1}
+let default_sigHashAlg pv cs =
+    default_sigHashAlg_fromSig pv (sigAlg_of_ciphersuite cs)
+
+let sigHashAlg_contains (algList:list Sig.alg) (alg:Sig.alg) =
+    List.existsb (fun a -> a = alg) algList
+
+let sigHashAlg_bySigList (algList:list Sig.alg) (sigAlgList:list sigAlg):list Sig.alg =
+    List.choose (fun alg -> let (sigA,_) = alg in if (List.existsb (fun a -> a = sigA) sigAlgList) then Some(alg) else None) algList
+
+let cert_type_to_SigHashAlg ct pv =
+    match ct with
+    | TLSConstants.DSA_fixed_dh | TLSConstants.DSA_sign -> default_sigHashAlg_fromSig pv DSA
+    | TLSConstants.RSA_fixed_dh | TLSConstants.RSA_sign -> default_sigHashAlg_fromSig pv RSASIG
+
+let rec cert_type_list_to_SigHashAlg ctl pv =
+    // FIXME: Generates a list with duplicates!
+    match ctl with
+    | [] -> []
+    | h::t -> (cert_type_to_SigHashAlg h pv) @ (cert_type_list_to_SigHashAlg t pv)
+
+let cert_type_to_SigAlg ct =
+    match ct with
+    | TLSConstants.DSA_fixed_dh | TLSConstants.DSA_sign -> DSA
+    | TLSConstants.RSA_fixed_dh | TLSConstants.RSA_sign -> RSASIG
+
+let rec cert_type_list_to_SigAlg ctl =
+    // FIXME: Generates a list with duplicates!
+    match ctl with
+    | [] -> []
+    | h::t -> (cert_type_to_SigAlg h) :: (cert_type_list_to_SigAlg t)
